RocqOfNoir/keccak/simulation.v
@@ -1,7 +1,7 @@
 Require Import RocqOfNoir.RocqOfNoir.
 Require Import RocqOfNoir.proof.RocqOfNoir.
 Require Import RocqOfNoir.simulation.RocqOfNoir.
-Require RocqOfNoir.keccak.polymorphic.
+Require Import RocqOfNoir.keccak.polymorphic.
 
 (* global BLOCK_SIZE_IN_BYTES: u32 = 136; *)
 Definition BLOCK_SIZE_IN_BYTES: Z := 136.
@@ -107,8 +107,259 @@ pub fn keccak256<let N: u32>(input: [u8; N], message_size: u32) -> [u8; 32] {
 }
 *)
 
-Definition keccak256
-    (is_unconstrained : bool)
-    {N : U32.t} (input : Array.t U8.t N) (message_size : U32.t) :
-    Array.t U8.t {| Integer.value := 32 |}.
+Parameter for_loop : forall {A : Set} (acc : A) (start end_ : Z) (body : A -> Z -> M! A), M! A.
+
+Lemma run_for_loop {State Address : Set} `{State.Trait State Address} (p : Z)
+    {A : Set} `{ToValue A}
+    (acc_in : A) (state_in : State)
+    (start end_ : Z)
+    (body : A -> Z -> M! A) (source_body : Z -> M.t)
+    (P_A : A -> State -> Prop)
+    (H_state_in : P_A acc_in state_in) :
+  (forall acc state i,
+    P_A acc state ->
+    let output := body acc i in
+    let P_state_out state_out :=
+      match output with
+      | Panic.Error => True
+      | Panic.Success acc_out =>
+        P_A acc_out state_out
+      end in
+    {{ p, state ⏩
+      source_body i 🔽
+      Panic.to_result (body acc i)
+    ⏩ P_state_out }}
+  ) ->
+  let output := for_loop acc_in start end_ body in
+  let P_state_out state_out :=
+    match output with
+    | Panic.Error => True
+    | Panic.Success acc_out =>
+      P_A acc_out state_out
+    end in
+  {{ p, state_in ⏩
+    M.for_Z start end_ source_body 🔽
+    Panic.to_result output
+  ⏩ P_state_out }}.
+Proof.
 Admitted.
+
+(* pub fn keccak256<let N: u32>(input: [u8; N], message_size: u32) -> [u8; 32] *)
+Definition keccak256 (p : Z) {N : U32.t}
+    (input : Array.t U8.t N) (message_size : U32.t) :
+    M! _ :=
+  (* assert(N >= message_size); *)
+  let! _ := Panic.assert (N.(Integer.value) >=? message_size.(Integer.value)) in
+
+  (*
+  let mut block_bytes = [0; ((N / BLOCK_SIZE_IN_BYTES) + 1) * BLOCK_SIZE_IN_BYTES];
+  if is_unconstrained() {
+      for i in 0..message_size {
+          block_bytes[i] = input[i];
+      }
+  } else {
+      for i in 0..N {
+          if i < message_size {
+              block_bytes[i] = input[i];
+          }
+      }
+  }
+  *)
+  let block_bytes : Array.t U8.t _ :=
+    Array.repeat
+      {| Integer.value := (N.(Integer.value) / BLOCK_SIZE_IN_BYTES + 1) * BLOCK_SIZE_IN_BYTES |}
+      {| Integer.value := 0 |} in
+  let! block_bytes :=
+    for_loop
+      block_bytes
+      0
+      message_size.(Integer.value)
+      (fun acc i =>
+        let! element := Array.read input i in
+        Array.write acc i element
+      ) in
+
+  (*
+  let max_blocks = (N + BLOCK_SIZE_IN_BYTES) / BLOCK_SIZE_IN_BYTES;
+  //maximum number of bytes to hash
+  let real_max_blocks = (message_size + BLOCK_SIZE_IN_BYTES) / BLOCK_SIZE_IN_BYTES;
+  let real_blocks_bytes = real_max_blocks * BLOCK_SIZE_IN_BYTES;
+  *)
+  let max_blocks := (N.(Integer.value) + BLOCK_SIZE_IN_BYTES) / BLOCK_SIZE_IN_BYTES in
+  let real_max_blocks := (message_size.(Integer.value) + BLOCK_SIZE_IN_BYTES) / BLOCK_SIZE_IN_BYTES in
+  let real_blocks_bytes := real_max_blocks * BLOCK_SIZE_IN_BYTES in
+
+  (*
+  block_bytes[message_size] = 1;
+  block_bytes[real_blocks_bytes - 1] = 0x80;
+  *)
+  let! block_bytes := Array.write block_bytes message_size.(Integer.value) {| Integer.value := 1 |} in
+  let! block_bytes := Array.write block_bytes (real_blocks_bytes - 1) {| Integer.value := 0x80 |} in
+
+  (*
+  let mut sliced_buffer =
+      [0; (((N / BLOCK_SIZE_IN_BYTES) + 1) * BLOCK_SIZE_IN_BYTES) / WORD_SIZE];
+  for i in 0..sliced_buffer.len() {
+      let limb_start = WORD_SIZE * i;
+
+      let mut sliced = 0;
+      let mut v = 1;
+      for k in 0..WORD_SIZE {
+          sliced += v * (block_bytes[limb_start + k] as Field);
+          v *= 256;
+      }
+
+      sliced_buffer[i] = sliced as u64;
+  }
+  *)
+  let sliced_buffer_len := (((N.(Integer.value) / BLOCK_SIZE_IN_BYTES) + 1) * BLOCK_SIZE_IN_BYTES) / WORD_SIZE in
+  let sliced_buffer : Array.t Field.t _ :=
+    Array.repeat
+      {| Integer.value := sliced_buffer_len |}
+      {| Field.value := 0 |} in
+  let! sliced_buffer :=
+    for_loop
+      sliced_buffer
+      0
+      sliced_buffer_len
+      (fun sliced_buffer i =>
+        let limb_start := WORD_SIZE * i in
+
+        let sliced := {| Field.value := 0 |} in
+        let v := {| Field.value := 1 |} in
+        let! (sliced, v) :=
+          for_loop
+            (sliced, v)
+            0
+            WORD_SIZE
+            (fun '(sliced, v) k =>
+              let! element := Array.read block_bytes (limb_start + k) in
+              let! element := Field.cast p element in
+              return! (
+                Field.add p sliced (Field.mul p v element),
+                Field.add p v {| Field.value := 256 |}
+            )
+            ) in
+        Array.write sliced_buffer i sliced
+      ) in
+
+  return! sliced_buffer.
+
+Module State.
+  Record t : Set := {
+    block_bytes : option Value.t;
+    sliced_buffer : option Value.t;
+    sliced : option Value.t;
+    v : option Value.t;
+  }.
+
+  Definition empty : t := {|
+    block_bytes := None;
+    sliced_buffer := None;
+    sliced := None;
+    v := None;
+  |}.
+End State.
+
+Module Address.
+  Inductive t : Set :=
+  | BlockBytes
+  | SlicedBuffer
+  | Sliced
+  | V.
+End Address.
+
+Instance Impl_State_for_State : State.Trait State.t Address.t := {
+  read state address :=
+    match address with
+    | Address.BlockBytes => state.(State.block_bytes)
+    | Address.SlicedBuffer => state.(State.sliced_buffer)
+    | Address.Sliced => state.(State.sliced)
+    | Address.V => state.(State.v)
+    end;
+  alloc_write state address value :=
+    match address with
+    | Address.BlockBytes => Some (state <| State.block_bytes := Some value |>)
+    | Address.SlicedBuffer => Some (state <| State.sliced_buffer := Some value |>)
+    | Address.Sliced => Some (state <| State.sliced := Some value |>)
+    | Address.V => Some (state <| State.v := Some value |>)
+    end;
+}.
+
+Lemma RunLetPanic {State Address : Set} `{State.Trait State Address} (p : Z)
+    {A B : Set} `{ToValue A} `{ToValue B}
+    (e : M.t) (e' : M! A)
+    (k : Result.t -> M.t) (k' : A -> M! B)
+    (state_in : State)
+    (P_state_inter P_state_out : State -> Prop) :
+  {{ p, state_in ⏩
+    e 🔽 Panic.to_result e'
+  ⏩ P_state_inter }} ->
+  (forall (state_inter : State) (output_inter : A),
+    P_state_inter state_inter ->
+    {{ p, state_inter ⏩
+      k (Result.Ok (to_value output_inter)) 🔽 Panic.to_result (k' output_inter)
+    ⏩ P_state_out }}
+  ) ->
+  (k Result.Panic = LowM.Pure Result.Panic) ->
+  P_state_out 
+  {{ p, state_in ⏩
+    LowM.Let e k 🔽 Panic.to_result (Panic.bind e' k')
+  ⏩ P_state_out }}.
+Proof.
+  intros H_e H_k H_k_panic.
+  eapply Run.Let; cbn. {
+    apply H_e.
+  }
+  intros state_inter H_state_inter.
+  destruct e'; cbn in *.
+  { now apply H_k. }
+  { rewrite H_k_panic.
+    apply Run.Pure.
+  }
+  eapply H_k.
+  - exact state_in.
+  - exact (to_value e').
+
+Lemma run_keccak256
+    (p : Z)
+    {N : U32.t}
+    (input : Array.t U8.t N) (message_size : U32.t)
+    (H_unconstrained :
+      [[ M.call_closure (|
+        M.read (| Builtin.is_unconstrained |),
+        []
+      |) ]] =
+      M.pure (Value.Bool true)
+    )
+    (H_message_size : message_size.(Integer.value) <= N.(Integer.value)) :
+  let output := keccak256 p input message_size in
+  let P_state_out state_out :=
+    match output with
+    | Panic.Error => True
+    | Panic.Success sliced_buffer =>
+      state_out.(State.sliced_buffer) = Some (to_value sliced_buffer)
+    end in
+  {{ p, State.empty ⏩
+    polymorphic.keccak256 N [to_value input; to_value message_size] 🔽
+    Panic.to_result output
+  ⏩ P_state_out }}.
+Proof.
+  unfold polymorphic.keccak256, keccak256.
+  progress repeat rewrite H_unconstrained.
+  eapply Run.Let; cbn. {
+    destruct (_ >=? _) eqn:?; [|lia]; cbn.
+    apply Run.PureExact.
+  }
+  intros ? ->; cbn.
+  eapply Run.Let; cbn. {
+    eapply Run.CallPrimitiveStateAlloc with (address := Address.BlockBytes); try reflexivity.
+    unfold set.
+    apply Run.PureExact.
+  }
+  intros ? ->; cbn.
+  eapply Run.Let; cbn. {
+    apply run_for_loop. with (acc_in :=).
+  cbn in H_unconstrained.
+  rewrite H_unconstrained; cbn.
+  cbn.
