RocqOfNoir/keccak/monomorphic.v
@@ -712,10 +712,10 @@ Definition keccak256₀ (α : list Value.t) : M.t :=
             |))
           |) ]] in
           let~ sliced := [[ M.copy_mutable (|
-            M.alloc (Value.Integer IntegerKind.Field 0)
+            M.alloc (Value.Field 0)
           |) ]] in
           let~ v := [[ M.copy_mutable (|
-            M.alloc (Value.Integer IntegerKind.Field 1)
+            M.alloc (Value.Field 1)
           |) ]] in
           do~ [[
             M.for_ (|
@@ -729,15 +729,14 @@ Definition keccak256₀ (α : list Value.t) : M.t :=
                     M.read (| sliced |),
                     Binary.multiply (|
                       M.read (| v |),
-                      M.cast (|
+                      M.cast_to_field (|
                         M.read (| M.index (|
                           block_bytes,
                           Binary.add (|
                             M.read (| limb_start |),
                             M.read (| k |)
                           |)
-                        |) |),
-                        IntegerKind.Field
+                        |) |)
                       |)
                     |)
                   |)
@@ -748,7 +747,7 @@ Definition keccak256₀ (α : list Value.t) : M.t :=
                   v,
                   Binary.multiply (|
                     M.read (| v |),
-                    Value.Integer IntegerKind.Field 256
+                    Value.Field 256
                   |)
                 |))
               ]]
@@ -1011,12 +1010,11 @@ Definition keccak256₀ (α : list Value.t) : M.t :=
           Value.Integer IntegerKind.U32 4,
           fun (i : Value.t) =>
           let~ lane := [[ M.copy (|
-            M.alloc (M.cast (|
+            M.alloc (M.cast_to_field (|
               M.read (| M.index (|
                 state,
                 M.read (| i |)
-              |) |),
-              IntegerKind.Field
+              |) |)
             |))
           |) ]] in
           let~ lane_le := [[ M.copy (|
